theories/tactics.v
@@ -54,6 +54,24 @@ Ltac unpack :=
       destruct h
     end.
 
+Ltac unzip :=
+  repeat match goal with
+  | [h: _ /\ _ |- _ ] =>
+    destruct h
+  | [h: _ \/ _ |- _ ] =>
+    destruct h
+  |[h: exists x, _ |- _] =>
+    let x := fresh x in
+    destruct h as [x h]
+  |[h: List.Forall _ (_ :: _) |- _] =>
+    inversion h;
+    subst;
+    clear h
+  |[h: List.Forall _ (_ ++ _) |- _] =>
+    rewrite List.Forall_app in h;
+    destruct h
+  end.
+
 Section unpack_tests.
   Example unpacking_forall_ex1 {A} (P: A -> Prop) l1 l2:
     List.Forall P (l1 ++ l2)
